To show the definition is reflexive, let $f: X \to Y$ be a function. We must to show $f=f$. Let $x \in X$. Then $f(x) = f(x)$ by reflexivity of equality on elements of $Y$. Since $x$ was arbitrary, this shows that $f=f$.

To show the defintion is symmetric, let $f: X \to Y$ and $g: X \to Y$ be two functions with the same domain and codomain. Suppose $f=g$. This means that $f(x) = g(x)$ for all $x \in X$. To show that $g = f$, we must show that $g(x) = f(x)$ for all $x \in X$. So let $x \in X$. Then since $f = g$ we have $f(x)=g(x)$. By symmetry of equality on the elements of $Y$, we have $g(x) = f(x)$. Since $x$ was arbitrary, this shows that $g = f$.

To show the defintion is transitive, let $f:X \to Y$, $g: X \to Y$ and $h: X \to Y$ be three functions with the same domain and codomain. Suppose $f = g$ and $g = h$. We must show $f = h$. So let $x \in X$. Then we have $f(x)=g(x)$ since $f=g$. We also have $g(x)=h(x)$ since $g=h$. By transitivity of equality on elements of $Y$, we have $f(x)=h(x)$. Since $x$ was arbitrary, this shows that $f = h$.

Now let $f,\tilde{f}: X \to Y$ and $g,\tilde{g}: Y \to Z$ be functions such that $f = \tilde{f}$ and $g = \tilde{g}$. We want to show $g \circ f = \tilde{g} \circ \tilde{f}$. Let $x \in X$. Then since $f = \tilde{f}$ we have $f(x) = \tilde{f}(x)$. By the substitution axiom of equality for elements of $Y$, we have $g(f(x)) = g(\tilde{f}(x))$. Since $g = \tilde{g}$, we have $g(\tilde{f}(x)) = \tilde{g}(\tilde{f}(x))$. Now we have $(g \circ f)(x) = g(f(x)) = g(\tilde{f}(x)) = \tilde{g}(\tilde{f}(x)) = (\tilde{g} \circ \tilde{f})(x)$ using symmetry and transitivity of equality on elements of $Z$. Since $x \in X$ was arbitrary, this shows that $g \circ f = \tilde{g} \circ \tilde{f}$ as required. <span style="float: right">â–¡</span> 